feat: rule out Reification

CollapsingTowers/TwoLevelPCP/Typing.lean
@@ -2,65 +2,65 @@
 import CollapsingTowers.TwoLevelPCP.Syntax
 import CollapsingTowers.TwoLevelPCP.SmallStep
 import CollapsingTowers.TwoLevelPCP.Env
-inductive typing : Stage → TEnv → Expr → Ty → Prop where
-  | fvar : ∀ 𝕊 Γ x τ,
+inductive typing : TEnv → Stage → Expr → Ty → Prop where
+  | fvar : ∀ Γ 𝕊 x τ,
     binds x τ 𝕊 Γ →
-    typing 𝕊 Γ (.fvar x) τ
-  | lam₁ : ∀ 𝕊 Γ e τ𝕒 τ𝕓,
-    typing 𝕊 ((τ𝕒, 𝕊) :: Γ) (open₀ Γ.length e) τ𝕓 →
-    binding_time 𝕊 τ𝕒 →
+    typing Γ 𝕊 (.fvar x) τ
+  | lam₁ : ∀ Γ 𝕊 e τ𝕒 τ𝕓,
+    typing ((τ𝕒, 𝕊) :: Γ) 𝕊 (open₀ Γ.length e) τ𝕓 →
+    well_binding_time 𝕊 τ𝕒 →
     closed_at e Γ.length →
-    typing 𝕊 Γ (.lam₁ e) (.arrow τ𝕒 τ𝕓)
+    typing Γ 𝕊 (.lam₁ e) (.arrow τ𝕒 τ𝕓)
   | lift_lam : ∀ Γ e τ𝕒 τ𝕓,
-    typing .fst Γ e (.arrow (.rep₁ τ𝕒) (.rep₁ τ𝕓)) →
-    typing .fst Γ (.lift e) (.rep₁ (.arrow τ𝕒 τ𝕓))
-  | app₁ : ∀ 𝕊 Γ f arg τ𝕒 τ𝕓,
-    typing 𝕊 Γ f (.arrow τ𝕒 τ𝕓) →
-    typing 𝕊 Γ arg τ𝕒 →
-    typing 𝕊 Γ (.app₁ f arg) τ𝕓
+    typing Γ .stat e (.arrow (.fragment τ𝕒) (.fragment τ𝕓)) →
+    typing Γ .stat (.lift e) (.fragment (.arrow τ𝕒 τ𝕓))
+  | app₁ : ∀ Γ 𝕊 f arg τ𝕒 τ𝕓,
+    typing Γ 𝕊 f (.arrow τ𝕒 τ𝕓) →
+    typing Γ 𝕊 arg τ𝕒 →
+    typing Γ 𝕊 (.app₁ f arg) τ𝕓
   | app₂ : ∀ Γ f arg τ𝕒 τ𝕓,
-    typing .fst Γ f (.rep₁ (.arrow τ𝕒 τ𝕓)) →
-    typing .fst Γ arg (.rep₁ τ𝕒) →
-    typing .fst Γ (.app₂ f arg) (.rep₁ τ𝕓)
-  | plus₁ : ∀ 𝕊 Γ l r,
-    typing 𝕊 Γ l .nat →
-    typing 𝕊 Γ r .nat →
-    typing 𝕊 Γ (.plus₁ l r) .nat
+    typing Γ .stat f (.fragment (.arrow τ𝕒 τ𝕓)) →
+    typing Γ .stat arg (.fragment τ𝕒) →
+    typing Γ .stat (.app₂ f arg) (.fragment τ𝕓)
+  | plus₁ : ∀ Γ 𝕊 l r,
+    typing Γ 𝕊 l .nat →
+    typing Γ 𝕊 r .nat →
+    typing Γ 𝕊 (.plus₁ l r) .nat
   | plus₂ : ∀ Γ l r,
-    typing .fst Γ l (.rep₁ .nat) →
-    typing .fst Γ r (.rep₁ .nat) →
-    typing .fst Γ (.plus₂ l r) (.rep₁ .nat)
-  | lit₁ : ∀ 𝕊 Γ n,
-    typing 𝕊 Γ (.lit₁ n) .nat
+    typing Γ .stat l (.fragment .nat) →
+    typing Γ .stat r (.fragment .nat) →
+    typing Γ .stat (.plus₂ l r) (.fragment .nat)
+  | lit₁ : ∀ Γ 𝕊 n,
+    typing Γ 𝕊 (.lit₁ n) .nat
   | lift_lit : ∀ Γ n,
-    typing .fst Γ n .nat →
-    typing .fst Γ (.lift n) (.rep₁ .nat)
+    typing Γ .stat n .nat →
+    typing Γ .stat (.lift n) (.fragment .nat)
   | code₁ : ∀ Γ x τ,
-    binds x τ .snd Γ →
-    typing .fst Γ (.code (.fvar x)) (.rep₁ τ)
+    binds x τ .dyn Γ →
+    typing Γ .stat (.code (.fvar x)) (.fragment τ)
   | code₂ : ∀ Γ e τ,
-    typing .snd Γ e τ →
-    typing .fst Γ (.code e) (.rep₂ τ)
+    typing Γ .dyn e τ →
+    typing Γ .stat (.code e) (.rep τ)
   | lift_code : ∀ Γ e τ,
-    typing .fst Γ e (.rep₁ τ) →
-    typing .fst Γ e (.rep₂ τ)
+    typing Γ .stat e (.fragment τ) →
+    typing Γ .stat e (.rep τ)
   | reflect : ∀ Γ e τ,
-    typing .snd Γ e τ →
-    typing .fst Γ (.reflect e) (.rep₁ τ)
+    typing Γ .dyn e τ →
+    typing Γ .stat (.reflect e) (.fragment τ)
   | lam𝕔 : ∀ Γ e τ𝕒 τ𝕓,
-    typing .fst ((τ𝕒, .snd) :: Γ) (open₀ Γ.length e) (.rep₂ τ𝕓) →
-    binding_time .snd τ𝕒 →
+    typing ((τ𝕒, .dyn) :: Γ) .stat (open₀ Γ.length e) (.rep τ𝕓) →
+    well_binding_time .dyn τ𝕒 →
     closed_at e Γ.length →
-    typing .fst Γ (.lam𝕔 e) (.rep₁ (.arrow τ𝕒 τ𝕓))
-  | lets : ∀ 𝕊 Γ b e τ𝕒 τ𝕓,
-    typing 𝕊 Γ b τ𝕒 →
-    typing 𝕊 ((τ𝕒, 𝕊) :: Γ) (open₀ Γ.length e) τ𝕓 →
-    binding_time 𝕊 τ𝕒 →
+    typing Γ .stat (.lam𝕔 e) (.fragment (.arrow τ𝕒 τ𝕓))
+  | lets : ∀ Γ 𝕊 b e τ𝕒 τ𝕓,
+    typing Γ 𝕊 b τ𝕒 →
+    typing ((τ𝕒, 𝕊) :: Γ) 𝕊 (open₀ Γ.length e) τ𝕓 →
+    well_binding_time 𝕊 τ𝕒 →
     closed_at e Γ.length →
-    typing 𝕊 Γ (.lets b e) τ𝕓
+    typing Γ 𝕊 (.lets b e) τ𝕓
   | let𝕔 : ∀ Γ b e τ𝕒 τ𝕓,
-    typing .snd Γ b τ𝕒 →
-    typing .fst ((τ𝕒, .snd) :: Γ) (open₀ Γ.length e) τ𝕓 →
-    binding_time .snd τ𝕒 →
+    typing Γ .dyn b τ𝕒 →
+    typing ((τ𝕒, .dyn) :: Γ) .stat (open₀ Γ.length e) (.rep τ𝕓) →
+    well_binding_time .dyn τ𝕒 →
     closed_at e Γ.length →
-    typing .fst Γ (.let𝕔 b e) τ𝕓
+    typing Γ .stat (.let𝕔 b e) (.rep τ𝕓)
